port reorder_malloc to expr_rel

theories/simplang/examples/reorder_malloc.v
@@ -1,4 +1,4 @@
-From simuliris.simplang Require Import lang notation tactics class_instances heap_bij heapbij_refl.
+From simuliris.simplang Require Import lang notation tactics class_instances heap_bij open_expr_rel.
 From iris.proofmode Require Import tactics.
 From simuliris.simulation Require Import slsls lifting.
 
@@ -7,28 +7,30 @@ From simuliris.simulation Require Import slsls lifting.
 Section reorder.
   Context `{sbijG Σ}.
 
-  Definition alloc2_and_cont :=
-    (λ: "a", let: "v1" := Fst "a" in
-             let: "v2" := Fst (Snd "a") in
-             let: "cont" := Snd (Snd "a") in
-             let: "l1" := Alloc "v1" in
-             let: "l2" := Alloc "v2" in
-             Call "cont" ("l1", "l2")
-    )%E.
+  Definition alloc2_and_cont : expr :=
+    let: "v1" := Fst "a" in
+    let: "v2" := Fst (Snd "a") in
+    let: "cont" := Snd (Snd "a") in
+    let: "l1" := Alloc "v1" in
+    let: "l2" := Alloc "v2" in
+    Call "cont" ("l1", "l2").
 
-  Definition alloc2_and_cont' :=
-    (λ: "a", let: "v1" := Fst "a" in
-             let: "v2" := Fst (Snd "a") in
-             let: "cont" := Snd (Snd "a") in
-             let: "l1" := Alloc "v2" in
-             let: "l2" := Alloc "v1" in
-             Call "cont" ("l2", "l1")
-    )%E.
+  Definition alloc2_and_cont' : expr :=
+    let: "v1" := Fst "a" in
+    let: "v2" := Fst (Snd "a") in
+    let: "cont" := Snd (Snd "a") in
+    let: "l1" := Alloc "v2" in
+    let: "l2" := Alloc "v1" in
+    Call "cont" ("l2", "l1").
 
-  Lemma alloc2_reorder π:
-    ⊢ sim_ectx val_rel π alloc2_and_cont alloc2_and_cont' val_rel.
+  Lemma alloc2_reorder :
+    ⊢ expr_rel alloc2_and_cont alloc2_and_cont'.
   Proof.
-    iIntros (v_t v_s) "Hrel". sim_pures.
+    iApply (expr_rel_subst "a").
+    iIntros (v_t v_s) "Hrel /=".
+    iApply expr_rel_closed; [compute_done..|]. iIntros (π).
+
+    sim_pures.
 
     source_bind (Fst v_s).
     iApply source_red_irred_unless; first done.
